Done with lemmas

src/Std/Data/HashMap/Basic.lean
@@ -274,6 +274,12 @@ instance [BEq α] [Hashable α] : Union (HashMap α β) := ⟨union⟩
 
 instance [BEq α] [Hashable α] : Inter (HashMap α β) := ⟨inter⟩
 
+/-- Internal implementation detail of the hash map. -/
+def beq {β : Type v} [BEq α] [BEq β] (m₁ m₂ : HashMap α β) : Bool :=
+  DHashMap.Const.beq m₁.inner m₂.inner
+
+instance [BEq α] [BEq β] : BEq (HashMap α β) := ⟨beq⟩
+
 section Unverified
 
 /-! We currently do not provide lemmas for the functions below. -/
