src/Std/Data/HashSet/Basic.lean
@@ -259,6 +259,12 @@ This function always iterates through the smaller set, so the expected runtime i
 
 instance [BEq α] [Hashable α] : Inter (HashSet α) := ⟨inter⟩
 
+/-- Internal implementation detail of the hash map. -/
+def beq [BEq α] (m₁ m₂ : HashSet α) : Bool :=
+  HashMap.beq m₁.inner m₂.inner
+
+instance [BEq α] : BEq (HashSet α) := ⟨beq⟩
+
 section Unverified
 
 /-! We currently do not provide lemmas for the functions below. -/
