src/Std/Data/HashMap/Lemmas.lean
@@ -1346,6 +1346,20 @@ theorem isEmpty_of_isEmpty_insertMany [EquivBEq α] [LawfulHashable α]
     {l : ρ} : (insertMany m l).isEmpty → m.isEmpty :=
   DHashMap.Const.isEmpty_of_isEmpty_insertMany
 
+section
+variable {β : Type v} {m₁ m₂ : HashMap α β} [BEq β]
+
+theorem Equiv.beq [LawfulHashable α] [EquivBEq α] [ReflBEq β] (h : m₁ ~m m₂) : m₁ == m₂ :=
+  DHashMap.Const.Equiv.beq h.1
+
+theorem Equiv_of_beq_eq_true [LawfulBEq α] [LawfulBEq β] (h : m₁ == m₂) : m₁ ~m m₂ :=
+  ⟨DHashMap.Const.Equiv_of_beq_eq_true h⟩
+
+theorem Equiv.beq_congr [LawfulBEq α] {m₃ m₄ : HashMap α β} : m₁ ~m m₃ → m₂ ~m m₄ → (m₁ == m₂) = (m₃ == m₄) := fun h1 h2 =>
+  DHashMap.Const.Equiv.beq_congr h1.1 h2.1
+
+end
+
 section Union
 variable {β : Type v}
 
